Watermarked_Stream_Antichain.thy
@@ -1,0 +1,108 @@
+theory Watermarked_Stream_Antichain
+  imports
+    "Antichain"
+    "Watermarked_Stream"
+begin
+
+definition "antichain_from_stream lxs =
+  (let xs = filter (\<lambda> ev. case ev of Data t d \<Rightarrow> \<not> (\<exists> wm. Watermark wm \<in> lset lxs \<and> t \<le> wm) | Watermark _ \<Rightarrow> False) (list_of lxs) in
+   let tss = map tmp xs in
+   maximal_antichain_list tss)"
+
+lemma list_of_lfilter_lfinite:
+  "lfinite lxs \<Longrightarrow>
+   list_of (lfilter P lxs) = filter P (list_of lxs)"
+  by (metis lfilter_llist_of list_of_llist_of llist_of_list_of)
+
+(* FIXME: move me *)
+lemma fun_to_case_event[simp]:
+  "(\<lambda>x. (\<forall>x11. (\<exists>x12. x = Data x11 x12) \<longrightarrow> P x11 \<and> (\<forall>wm. Watermark wm \<in> lset lxs \<longrightarrow> \<not> x11 \<le> wm)) \<and> (\<forall>x2. x \<noteq> Watermark x2)) = 
+   case_event (\<lambda>t' d. P t' \<and> (\<forall>wm. Watermark wm \<in> lset lxs \<longrightarrow> \<not> t' \<le> wm)) (\<lambda>x. False)"
+  apply (rule ext)
+  apply (auto split: event.splits)
+  done
+
+(* FIXME: move me *)
+lemma filter_map_filter[simp]:
+  "filter P (List.map_filter Q xs) = List.map_filter (\<lambda> x. case Q x of Some y \<Rightarrow> (if P y then Some y else None) | None \<Rightarrow> None) xs"
+  apply (induct xs)
+   apply (auto simp add: map_filter_simps split: option.splits)
+  done
+
+lemma antichain_from_stream_Cons_Data:
+  "lfinite lxs \<Longrightarrow>
+   antichain_from_stream (LCons (Data t d) lxs) = (
+   if \<not> (\<exists> wm. Watermark wm \<in> lset lxs \<and> t \<le> wm) \<and> \<not> (\<exists> t' d. Data t' d \<in> lset lxs \<and> t' > t) 
+   then t # antichain_from_stream (lfilter (\<lambda> ev. case ev of Data t' _ \<Rightarrow> \<not> t' \<le> t | Watermark _ \<Rightarrow> True) lxs)
+   else antichain_from_stream lxs)"
+  apply (auto split: if_splits)
+  subgoal
+    unfolding antichain_from_stream_def Let_def
+    apply (auto 0 0 simp add: list_of_lfilter_lfinite Let_def split: event.splits)
+     apply (meson dual_order.strict_iff_not event.exhaust)
+    apply (simp flip: maximal_antichain_filter)
+    apply (rule arg_cong[where f="maximal_antichain_list"])
+    apply (simp add: map_filter_map_filter flip: )
+    unfolding  List.map_filter_def
+    apply auto
+    apply (rule map_cong)
+     apply (rule filter_cong)
+      apply simp
+     apply (auto split: event.splits)
+    done
+  subgoal
+    unfolding antichain_from_stream_def Let_def
+    apply (auto simp add:  split: event.splits)
+    done
+  subgoal for t' d
+    apply (cases "\<exists> wm. Watermark wm \<in> lset lxs \<and> t \<le> wm")
+    subgoal
+      apply (elim exE conjE)
+      unfolding antichain_from_stream_def Let_def
+      apply (auto simp add:  split: event.splits)
+      done
+    subgoal
+      unfolding antichain_from_stream_def Let_def
+      apply (subst (1 2) maximal_antichain_remove[where t=t' and t'=t])
+      subgoal
+        apply auto
+        apply (smt (verit, best) dual_order.order_iff_strict dual_order.trans event.sel(1) event.simps(5) imageI mem_Collect_eq)
+        done
+      subgoal
+        apply auto
+        apply (smt (verit, best) dual_order.order_iff_strict dual_order.trans event.sel(1) event.simps(5) imageI mem_Collect_eq)
+        done
+      subgoal
+        apply (auto simp add: list_of_lfilter_lfinite split: event.splits simp flip: maximal_antichain_filter)
+        done
+      done
+    done
+  done
+
+definition "ws_2 lxs wm = {wm'. wm' \<in> set (takeWhile ((\<noteq>) wm) (antichain_from_stream lxs))}"
+
+lemma ws_2_LCons_Data[simp]:
+  "lfinite lxs \<Longrightarrow>
+   ws_2 (LCons (Data t d) lxs) wm = (
+   if (\<nexists>wm. Watermark wm \<in> lset lxs \<and> t \<le> wm) \<and> (\<nexists>t' d. Data t' d \<in> lset lxs \<and> t < t')
+   then (if t = wm then {} else insert t (ws_2 (lfilter (\<lambda>x. case x of Data t' x \<Rightarrow> \<not> t' \<le> t | Watermark x \<Rightarrow> True) lxs) wm))
+   else ws_2 lxs wm)"
+  unfolding ws_2_def
+  apply (auto simp add: antichain_from_stream_Cons_Data split: if_splits)
+  done
+
+
+lemma antichain_from_stream_llist_of_map[simp]:
+  "antichain_from_stream (llist_of (map (\<lambda>(x, y). Data x y) buf)) = maximal_antichain_list (map fst buf)"
+  unfolding antichain_from_stream_def Let_def
+  apply (auto simp add: split_beta split: event.splits  prod.splits)
+  apply (rule arg_cong[where f=maximal_antichain_list])
+  apply (induct buf)
+   apply simp
+  subgoal for a buf'
+    apply (cases a)
+    apply auto
+    done
+  done
+
+end
